coq/proof/SoundSnapshot.v
@@ -17,6 +17,7 @@ Import Opsem.
 Require Import TODO.
 Require Import Validator.
 Require Import Postcond.
+Require Import Exprs.
 Require Import GenericValues.
 Require InvMem.
 Require InvState.
@@ -24,11 +25,49 @@ Require Import SoundBase.
 
 Set Implicit Arguments.
 
-Lemma snapshot_sound
-      conf_src conf_tgt st_src st_tgt invst0 invmem0 inv0 inv1
-      (STATE: InvState.Rel.sem conf_src conf_tgt st_src st_tgt invst0 invmem0 inv0)
-      (SNAPSHOT: Snapshot.t inv0 = inv1):
-  exists invst1,
-    <<STATE: InvState.Rel.sem conf_src conf_tgt st_src st_tgt invst1 invmem0 inv1>>.
+
+(* TODO: lemma on tag.previous *)
+
+Definition snapshot_as_previous st invst: Prop :=
+  forall x gvx
+         (LOCAL_IN: lookupAL _ st.(EC).(Locals) x = Some gvx),
+    <<PREV: InvState.Unary.sem_idT st invst (Tag.previous, x) = Some gvx>>.
+
+Lemma snapshot_unary_sound
+      conf st invst0 invmem inv0
+      (STATE: InvState.Unary.sem conf st invst0 invmem inv0)
+  :
+    exists invst1,
+      <<STATE: InvState.Unary.sem conf st invst1 invmem (Snapshot.unary inv0)>> /\
+               <<PREV: snapshot_as_previous st invst1>>.
 Proof.
+Admitted.
+
+Lemma snapshot_sound
+      conf_src conf_tgt st_src st_tgt invst0 invmem inv0
+      (STATE: InvState.Rel.sem conf_src conf_tgt st_src st_tgt invst0 invmem inv0):
+  exists invst1,
+    <<STATE: InvState.Rel.sem conf_src conf_tgt st_src st_tgt invst1 invmem (Snapshot.t inv0)>> /\
+    <<PREV_SRC: snapshot_as_previous st_src invst1.(InvState.Rel.src)>> /\
+    <<PREV_TGT: snapshot_as_previous st_tgt invst1.(InvState.Rel.tgt)>>.
+Proof.
+  inv STATE.
+  apply snapshot_unary_sound in SRC.
+  apply snapshot_unary_sound in TGT. des.
+  esplits.
+  - econs.
+    + admit.
+    + admit.
+    + admit.
+      (* Lemma snapshot_maydiff_incr *)
+      (*       Snapshot.IdTSet maydiff *)
+
+
+
+    
+  
+
+
+
+  
 Admitted.
