coq/proof/SoundPostcondPhinodes.v
@@ -19,7 +19,13 @@ Require Import Validator.
 Require Import GenericValues.
 Require InvMem.
 Require InvState.
+Require Import Inject.
 Require Import SoundBase.
+Require Import SoundSnapshot.
+Require Import SoundForget.
+Require Import SoundReduceMaydiff.
+Require Import SoundImplies.
+(* Require Import SoundPhinodesAddLessdef. *)
 
 Set Implicit Arguments.
 
@@ -67,11 +73,206 @@ Lemma add_terminator_cond_br
 Proof.
 Admitted.
 
+(* TODO: position *)
+Ltac solve_match_bool :=
+  repeat (let MATCH := fresh "MATCH" in
+          match goal with
+          | [H:match ?c with _ => _ end = true |- _] =>
+            destruct c eqn:MATCH; try done
+          | [H:match ?c with _ => _ end = false |- _] =>
+            destruct c eqn:MATCH; try done
+          | [H:match ?c with | Some _ => _ | None => _ end =
+               Some _ |- _] =>
+            destruct c eqn:MATCH; try done
+          | [H:match ?c with | Some _ => _ | None => _ end =
+               None |- _] =>
+            destruct c eqn:MATCH; try done
+          | [H:if ?c then Some _ else None = Some _ |- _] =>
+            destruct c eqn:MATCH; try done
+          | [H:if ?c then Some _ else None = None |- _] =>
+            destruct c eqn:MATCH; try done
+          | [H:if ?c then None else Some _ = Some _ |- _] =>
+            destruct c eqn:MATCH; try done
+          | [H:if ?c then None else Some _ = None |- _] =>
+            destruct c eqn:MATCH; try done
+          end).
+
+(* TODO: move and prove*)
+Lemma get_lessdef_spec
+      ep assigns
+      (IN: Exprs.ExprPairSet.In ep (Postcond.Phinode.get_lessdef assigns)):
+  exists phix phiv phity,
+    <<IN: In (Postcond.Phinode.assign_intro phix phity phiv) assigns>> /\
+          (<<PAIR1: ep = (Exprs.Expr.value (Exprs.ValueT.id (Exprs.Tag.physical, phix)),
+                          Exprs.Expr.value (Exprs.ValueT.lift Exprs.Tag.previous phiv))>> \/
+           <<PAIR2: ep = (Exprs.Expr.value (Exprs.ValueT.lift Exprs.Tag.previous phiv),
+                          Exprs.Expr.value (Exprs.ValueT.id (Exprs.Tag.physical, phix)))>>).
+Proof.
+Admitted.
+
+Lemma phinode_assign_sound
+      conf phinodes b assigns
+      locals locals'
+      x ty v
+      (ASSIGNS: forallb_map (Postcond.Phinode.resolve (fst b)) phinodes = Some assigns)
+      (LOCALS': getIncomingValuesForBlockFromPHINodes
+                  conf.(CurTargetData) phinodes b conf.(Globals) locals = Some locals')
+      (UNIQUE_PHI: unique id_dec (List.map Postcond.Phinode.get_def assigns) = true)
+      (ASSIGN_IN: In (Postcond.Phinode.assign_intro x ty v) assigns)
+  :
+    exists gv,
+      <<VAL_V: getOperandValue conf.(CurTargetData) v locals conf.(Globals) = Some gv>> /\
+               <<VAL_X: getOperandValue conf.(CurTargetData) (value_id x) locals' conf.(Globals) = Some gv>>.
+Proof.
+  revert assigns locals locals' x ty v ASSIGNS LOCALS' UNIQUE_PHI ASSIGN_IN.
+  induction phinodes.
+  - i. ss. inv ASSIGNS. ss.
+  - i. ss.
+    simtac. des.
+    + inv ASSIGN_IN.
+      assert (EQV: v = v0).
+      { match goal with
+        | [H1: getValueViaBlockFromValuels _ _ = Some v0,
+           H2: lookupAL _ _ _ = Some v |- _] => clear -H1 H2
+        end.
+        unfold getValueViaBlockFromValuels in *.
+        induction l0; ss; simtac.
+        exploit IHl0; eauto.
+      }
+      subst. esplits; eauto.
+      match goal with
+      | [H:_ |- (if ?c then _ else _) = _ ] => destruct c; try done
+      end.
+    + exploit IHphinodes; eauto. i. des.
+      esplits; eauto.
+      destruct (id_dec x id5).
+      { subst.
+        assert (IN_DEFS: In id5 (List.map Postcond.Phinode.get_def l2)).
+        { replace id5 with (Postcond.Phinode.get_def (Postcond.Phinode.assign_intro id5 ty v)); eauto.
+          apply In_map; eauto.
+        }
+        destruct (in_dec id_dec id5 (List.map Postcond.Phinode.get_def l2)); done.
+      }
+      match goal with
+      | [H:_ |- (if ?c then _ else _) = _ ] => destruct c; try done
+      end.
+Qed.
+
+Lemma phinodes_add_lessdef_sound
+      conf st0 st1
+      l_to phinodes cmds terminator
+      invst invmem inv0
+      assigns
+      (STEP: switchToNewBasicBlock conf.(CurTargetData)
+                                          (l_to, stmts_intro phinodes cmds terminator)
+                                          st0.(EC).(CurBB)
+                                          conf.(Globals)
+                                          st0.(EC).(Locals) = Some st1.(EC).(Locals))
+      (ASSIGNS: forallb_map (Postcond.Phinode.resolve st0.(EC).(CurBB).(fst)) phinodes = Some assigns)
+      (UNIQUE_PHI: unique id_dec (List.map Postcond.Phinode.get_def assigns) = true)
+      (STATE: InvState.Unary.sem conf st1 invst invmem inv0)
+      (PREV: snapshot_as_previous st0 invst)
+  :
+  InvState.Unary.sem
+    conf st1 invst invmem
+    (Hints.Invariant.update_lessdef (Postcond.postcond_phinodes_add_lessdef assigns) inv0).
+Proof.
+  (* TODO: invst's previous = st0.(EC).(Locals) *)
+  inv STATE.
+  econs; eauto.
+  ss. unfold Postcond.postcond_phinodes_add_lessdef.
+  ii. exploit Exprs.ExprPairSet.union_1; eauto. i. des.
+  { exploit LESSDEF; eauto. }
+  clear LESSDEF NOALIAS UNIQUE PRIVATE H.
+  exploit get_lessdef_spec; eauto. i. des.
+  { subst. ss.
+    esplits; try reflexivity.
+    unfold switchToNewBasicBlock in *.
+    solve_match_bool. inv STEP. ss.
+    destruct (CurBB (EC st0)). ss.
+    exploit phinode_assign_sound; eauto; ss. i. des. ss.
+    exploit opsem_props.OpsemProps.updateValuesForNewBlock_spec4; eauto.
+    match goal with
+    | [H: updateValuesForNewBlock _ _ = _ |- _] => rewrite H; i
+    end.
+    assert (GV_VAL1: gv = val1).
+    { unfold InvState.Unary.sem_idT in VAL1. ss. congruence. }
+    subst.
+    unfold getOperandValue in VAL_V.
+    destruct phiv; eauto.
+    exploit PREV; eauto.
+  }
+  { subst. ss.
+    esplits; try reflexivity.
+    unfold switchToNewBasicBlock in *.
+    solve_match_bool. inv STEP. ss.
+    destruct (CurBB (EC st0)). ss.
+    exploit phinode_assign_sound; eauto; ss. i. des. ss.
+    exploit opsem_props.OpsemProps.updateValuesForNewBlock_spec4; eauto. 
+    match goal with
+    | [H: updateValuesForNewBlock _ _ = _ |- _] => rewrite H; i
+    end.
+    assert (GV_VAL1: gv = val1).
+    { unfold InvState.Unary.sem_idT. ss.
+      destruct phiv.
+      - exploit PREV; eauto. i. des.
+        ss. unfold InvState.Unary.sem_idT in *. ss. congruence.
+      - ss. congruence.
+    }
+    subst. eauto.
+  }
+Qed.
+
+Lemma phinodes_progress_getPhiNodeID_safe
+      TD phinodes b gl locals locals' id assigns
+      (GETINC: getIncomingValuesForBlockFromPHINodes TD phinodes b
+                                                     gl locals = Some locals')
+      (IN: In id (List.map getPhiNodeID phinodes))
+      (RESOLVE : forallb_map (Postcond.Phinode.resolve (fst b)) phinodes = Some assigns)
+  :
+    <<IN: In id (List.map Postcond.Phinode.get_def assigns)>>.
+Proof.
+  revert locals locals' id assigns GETINC IN RESOLVE.
+  induction phinodes; ss.
+  i. simtac.
+  des; eauto.
+  exploit IHphinodes; eauto.
+Qed.
+
+Lemma locals_equiv_after_phinode
+      conf l_to phinodes cmds tmn b assigns
+      locals locals'
+      (SWITCH: switchToNewBasicBlock conf.(CurTargetData) (l_to, stmts_intro phinodes cmds tmn)
+                                                          b conf.(Globals) locals = Some locals')
+      (RESOLVE: forallb_map (Postcond.Phinode.resolve b.(fst)) phinodes = Some assigns)
+  :
+    <<EQUIV: locals_equiv_except (Exprs.IdTSet_from_list (List.map (Exprs.IdT.lift Exprs.Tag.physical)
+                                                                   (List.map Postcond.Phinode.get_def assigns)))
+                                 locals locals'>>.
+Proof.
+  unfold locals_equiv_except. ii.
+  unfold switchToNewBasicBlock in SWITCH.
+  simtac.
+  apply opsem_props.OpsemProps.updateValuesForNewBlock_spec5; eauto.
+  destruct (in_dec id_dec id0 (List.map Postcond.Phinode.get_def assigns)).
+  { exfalso. apply NOT_IN.
+    apply Exprs.IdTSet.mem_2.
+    eapply Exprs.IdTSet_from_list_spec.
+    apply In_map. eauto.
+  }
+
+  destruct (in_dec id_dec id0 (List.map getPhiNodeID phinodes)).
+  { exploit phinodes_progress_getPhiNodeID_safe; eauto; done. }
+  hexploit opsem_props.OpsemProps.getIncomingValuesForBlockFromPHINodes_spec8; eauto. i.
+  exploit notin_lookupAL_None; eauto.
+Qed.
+
 Lemma postcond_phinodes_sound
-      conf_src st0_src phinodes_src cmds_src terminator_src locals_src
-      conf_tgt st0_tgt phinodes_tgt cmds_tgt terminator_tgt locals_tgt
+      m_src conf_src st0_src phinodes_src cmds_src terminator_src locals_src
+      m_tgt conf_tgt st0_tgt phinodes_tgt cmds_tgt terminator_tgt locals_tgt
       invst0 invmem inv0 inv1
       l_from l_to
+      (CONF: valid_conf m_src m_tgt conf_src conf_tgt)
       (CMD_SRC: st0_src.(EC).(CurCmds) = [])
       (CMD_TGT: st0_tgt.(EC).(CurCmds) = [])
       (L_SRC: st0_src.(EC).(CurBB).(fst) = l_from)
@@ -122,4 +323,36 @@ Lemma postcond_phinodes_sound
                   st0_tgt.(Mem))
                invst1 invmem inv1>>.
 Proof.
-Admitted.
+  unfold Postcond.postcond_phinodes in *.
+  unfold Postcond.postcond_phinodes_assigns in *.
+  simtac.
+  exploit snapshot_sound; eauto. i. des.
+  exploit forget_sound; eauto.
+  { instantiate (1 := mkState (mkEC _ _ _ _ _ _) _ _). econs; s.
+    - eauto.
+    - instantiate (1 := locals_src).
+      eapply locals_equiv_after_phinode; eauto.
+  }
+  { instantiate (1 := mkState (mkEC _ _ _ _ _ _) _ _). econs; s.
+    - eauto.
+    - instantiate (1 := locals_tgt).
+      eapply locals_equiv_after_phinode; eauto.
+      rewrite L_TGT. eauto.
+  }
+  i. des.
+  inversion x0.
+  exploit phinodes_add_lessdef_sound; try exact SRC; eauto. i.
+  exploit phinodes_add_lessdef_sound; try exact TGT; eauto.
+  { rewrite L_TGT. eauto. }
+  i. exploit reduce_maydiff_sound.
+  { eauto. }
+  { instantiate (1 := Hints.Invariant.mk _ _ _).
+    econs; s.
+    - apply x1.
+    - apply x2.
+    - eauto.
+  }
+  { eauto. }
+  s. i. des.
+  esplits; try exact STATE1; eauto.
+Qed.
